ML_SP_Inference.v
@@ -92,10 +92,6 @@ Qed.
 Definition unify K T1 T2 S :=
   unify (1 + size_pairs S K ((T1,T2)::nil)) ((T1,T2)::nil) K S.
 
-Definition fvs S K E T Ts :=
-  dom S \u fv_in typ_fv S \u dom K \u fv_in kind_fv K \u env_fv E
-  \u typ_fv_list (T :: Ts).
-
 (** Variants looking up a kinding environment *)
 
 Fixpoint close_fvars (n:nat)(K:kenv)(VK:vars)(Vs:vars) {struct n} : vars :=
@@ -130,8 +126,11 @@ Fixpoint typ_generalize (Bs:list var) (T:typ) {struct T} : typ :=
     typ_arrow (typ_generalize Bs T1) (typ_generalize Bs T2)
   end.
 
-Definition sch_generalize Bs T Ks :=
-  Sch (typ_generalize Bs T) (List.map (kind_map (typ_generalize Bs)) Ks).
+Definition presch := (typ * list kind)%type.
+Definition preenv := env presch.
+
+Definition sch_generalize Bs T Ks : presch :=
+  (typ_generalize Bs T, List.map (kind_map (typ_generalize Bs)) Ks).
 
 Fixpoint split_env (A:Set) (B:vars) (E:env A) {struct E} : env A * env A :=
   match E with
@@ -144,8 +143,22 @@ Fixpoint split_env (A:Set) (B:vars) (E:env A) {struct E} : env A * env A :=
 Definition vars_subst S L :=
   typ_fv_list (List.map (fun x => typ_subst S (typ_fvar x)) (S.elements L)).
 
+Definition pre_fv (p:presch) :=
+  typ_fv (fst p) \u kind_fv_list (snd p).
+
+Definition pre_subst S (p:presch) : presch :=
+  (typ_subst S (fst p), List.map (kind_subst S) (snd p)).
+
+Definition strip_pre M : presch := (sch_type M, sch_kinds M).
+Definition strip_env (E:Defs.env) :=
+  List.map (fun p:var*sch => (fst p, strip_pre (snd p))) E.
+
+Definition fvs S K E T Ts :=
+  dom S \u fv_in typ_fv S \u dom K \u fv_in kind_fv K \u fv_in pre_fv E
+  \u typ_fv_list (T :: Ts).
+
 Definition typinf_generalize K' E' L T1 :=
-  let ftve := close_fvk K' (env_fv E') in
+  let ftve := close_fvk K' (fv_in pre_fv E') in
   let (K'', KA) := split_env ftve K' in
   let B := close_fvk K' (typ_fv T1) in
   let (_, KB) := split_env B K'' in
@@ -155,7 +168,7 @@ Definition typinf_generalize K' E' L T1 :=
   let (_, KC) := split_env L K'' in
   (KA & KC, sch_generalize (Bs++Bs') T1 (Ks++Ks')).
 
-Fixpoint typinf (K:kenv) (E:Defs.env) (t:trm) (T:typ) (Ts:list typ) (S:subs)
+Fixpoint typinf (K:kenv) (E:preenv) (t:trm) (T:typ) (Ts:list typ) (S:subs)
   (h:nat) {struct h} : option (kenv * subs) :=
   match h with
   | 0 => None
@@ -166,8 +179,8 @@ Fixpoint typinf (K:kenv) (E:Defs.env) (t:trm) (T:typ) (Ts:list typ) (S:subs)
     match get x E with
     | None => None
     | Some M =>
-      let Vs := proj1_sig (var_freshes (fvs S K E T Ts) (sch_arity M)) in
-      unify (K & kinds_open_vars (sch_kinds M) Vs) (M ^ Vs) T S
+      let Vs := proj1_sig (var_freshes (fvs S K E T Ts) (length (snd M))) in
+      unify (K & kinds_open_vars (snd M) Vs) (typ_open_vars (fst M) Vs) T S
     end
   | trm_abs t1 =>
     let x := proj1_sig (var_fresh (dom E \u trm_fv t1)) in
@@ -176,7 +189,7 @@ Fixpoint typinf (K:kenv) (E:Defs.env) (t:trm) (T:typ) (Ts:list typ) (S:subs)
     match unify K (typ_arrow (typ_fvar v1) V2) T S with
     | None => None
     | Some (K',S') =>
-      typinf K' (E & x ~ Sch (typ_fvar v1) nil) (t1 ^ x) V2 (T::Ts) S' h'
+      typinf K' (E & x ~ (typ_fvar v1, nil)) (t1 ^ x) V2 (T::Ts) S' h'
     end
   | trm_let t1 t2 =>
     let V := typ_fvar (proj1_sig (var_fresh (fvs S K E T Ts))) in
@@ -184,7 +197,7 @@ Fixpoint typinf (K:kenv) (E:Defs.env) (t:trm) (T:typ) (Ts:list typ) (S:subs)
     | None => None
     | Some (K0,S') =>
       let K' := Env.map (kind_subst S') K0 in
-      let E' := Env.map (sch_subst S') E in
+      let E' := Env.map (pre_subst S') E in
       let T1 := typ_subst S' V in
       let (KA, M) := typinf_generalize K' E' (vars_subst S' (dom K)) T1 in
       let x := proj1_sig (var_fresh (dom E \u trm_fv t1 \u trm_fv t2)) in
@@ -224,6 +237,24 @@ Proof.
   subst.
   apply* typ_subst_type.
 Qed.
+
+Section EnvProp.
+  Variables (A:Set) (P:A->Prop).
+
+  Lemma env_prop_single : forall x a, P a -> env_prop P (x ~ a).
+  Proof.
+    intros; intro; intros.
+    destruct* H0.
+    inversions* H0.
+  Qed.
+
+  Lemma env_prop_concat : forall l1 l2,
+    env_prop P l1 -> env_prop P l2 -> env_prop P (l1 & l2).
+  Proof.
+    intros; intro; intros.
+    destruct* (in_app_or _ _ _ H1).
+  Qed.
+End EnvProp.
 
 Hint Resolve env_prop_single env_prop_concat env_prop_type_compose.
 
@@ -434,33 +465,43 @@ Proof.
   split*.
 Qed.
 
-Lemma proper_instance_well_subst : forall S K K' Ks Us,
-  env_prop type S ->
+Lemma proper_instance_well_subst : forall S HS K K' M Us,
   well_subst K K' S ->
   kenv_ok K' ->
-  proper_instance K Ks Us ->
-  proper_instance K' (List.map (kind_subst S) Ks) (List.map (typ_subst S) Us).
+  proper_instance K M Us ->
+  proper_instance K' (@sch_subst S HS M) (List.map (typ_subst S) Us).
 Proof.
   intros.
-  destruct H2 as [HUs HW].
+  destruct H1 as [HUs HW].
+  destruct M as [T Ks HM].
   split.
+    unfold sch_arity; simpl.
     destruct HUs.
     split. repeat rewrite map_length. auto.
-    clear -H H3.
-    induction H3; simpl*.
+    clear -HS H2.
+    induction H2; simpl*.
   pose (Ts := Us).
   assert (Us = Ts) by simpl*. clearbody Ts.
   pattern Us at 2.
   pattern Us at 2 in HW.
-  rewrite H2 in *.
-  clear H2.
+  rewrite H1 in *.
+  unfold sch_arity in *; simpl in *.
+  clear H1 HM.
   destruct HUs.
-  gen Ks; induction H3; destruct Ks; simpl; intros; try discriminate. auto.
+  gen Ks; induction H2; destruct Ks; simpl; intros; try discriminate. auto.
   split*.
   destruct HW.
-  clear IHlist_forall H6.
+  clear IHlist_forall H5.
   rewrite* <- kind_subst_open.
   apply* well_kinded_subst.
+Qed.
+
+Lemma All_kind_types_subst : forall k S,
+  All_kind_types type k ->
+  env_prop type S -> All_kind_types type (kind_subst S k).
+Proof.
+  intros; unfold kind_subst; apply All_kind_types_map.
+  apply* All_kind_types_imp.
 Qed.
 
 Lemma kenv_ok_map : forall K S,
@@ -483,24 +524,12 @@ Lemma kenv_ok_subst : forall K' K Ks Ys S,
   kenv_ok (K' & map (kind_subst S) (kinds_open_vars Ks Ys)).
 Proof.
   introv TS HK HK' Fr.
-  destruct (kenv_ok_concat_inv _ _ HK).
-  use (kenv_ok_map H0 TS).
-  split*.
+  apply* kenv_ok_concat.
+    destruct (kenv_ok_concat_inv _ _ HK).
+    apply* kenv_ok_map.
+  rewrite dom_map. rewrite* dom_kinds_open_vars.
+  apply* (fresh_disjoint (length Ks)).
 Qed.
-
-Lemma env_ok_map : forall E S,
-  env_ok E -> env_prop type S -> env_ok (map (sch_subst S) E).
-Proof.
-  intros; split*.
-  intro; intros.
-  destruct (in_map_inv _ _ _ _ H1) as [b [Hb B]].
-  subst.
-  Search scheme.
-  apply* sch_subst_type.
-  apply* (proj2 H x).
-Qed.
-
-Hint Resolve kenv_ok_subst env_ok_map.
 
 Lemma well_subst_extend : forall K S K' Ks Ys,
   env_prop type S ->
@@ -538,52 +567,55 @@ Proof.
   destruct* (fresh_disjoint _ _ _ Fr Z).
 Qed.
 
-Lemma typing_typ_well_subst : forall gc S K K' E t T,
-  env_prop type S ->
+Lemma typing_typ_well_subst : forall gc S TS K K' E t T,
   well_subst K K' S ->
   kenv_ok K' ->
   K ; E |gc|= t ~: T -> 
-  K'; map (sch_subst S) E |gc|= t ~: (typ_subst S T).
+  K'; map (@sch_subst S TS) E |gc|= t ~: (typ_subst S T).
 Proof.
-  introv TS WS HK' Typ.
+  introv WS HK' Typ.
   gen K'; induction Typ; intros.
   (* Var *)
-  rewrite~ sch_subst_open. apply* typing_var.
-  destruct M as [T Ks]; simpl in *.
+  rewrite~ (sch_subst_open TS). apply* typing_var.
   apply* proper_instance_well_subst.
   (* Abs *)
   simpl.
   apply_fresh* (@typing_abs gc) as y.
-  replace (Sch (typ_subst S U) nil) with (sch_subst S (Sch U nil)) by auto.
+  instantiate (1 := typ_subst_type TS HU).
+  replace (Sch_nil (typ_subst_type TS HU)) with (sch_subst TS (Sch_nil HU))
+    by apply* sch_eq.
   assert (y \notin L) by auto.
-  use (H1 _ H2 _ WS HK').
+  use (H0 _ H1 _ WS HK').
   (* Let *)
-  apply_fresh* (@typing_let gc (sch_subst S M)
+  apply_fresh* (@typing_let gc (sch_subst TS M)
     (L1 \u dom S \u fv_in typ_fv S \u sch_fv M \u dom K \u dom K')) as y.
     clear H1 H2. clear L2 T2 t2.
-    simpl. intros Ys Fr.
-    destruct M as [T Ks]; simpl in *.
+    destruct M as [T Ks HM].
+    intros Ys Fr.
+    unfold sch_arity in *; simpl in Fr, H0.
     rewrite map_length in Fr.
     assert (HK: kenv_ok (K & kinds_open_vars Ks Ys)).
       assert (fresh L1 (length Ks) Ys) by auto*.
+      simpl in H.
       use (H _ H1).
-    rewrite* <- sch_subst_open_vars.
+    rewrite* <- (sch_subst_open_vars TS).
+    simpl sch_kinds.
     rewrite* <- kinds_subst_open_vars.
     apply* H0; clear H H0.
-    apply* well_subst_extend.
-  replace (y ~ sch_subst S M) with (map (sch_subst S) (y ~ M)) by simpl*.
+      apply* well_subst_extend.
+    apply* kenv_ok_subst.
+  replace (y ~ sch_subst TS M) with (map (sch_subst TS) (y ~ M)) by simpl*.
   rewrite <- map_concat.
   apply* H2.
   (* App *)
   simpl in IHTyp1; auto*.
   (* Cst *)
-  rewrite* sch_subst_open.
+  rewrite* (sch_subst_open TS).
   assert (disjoint (dom S) (sch_fv (Delta.type c))).
     intro x. rewrite* Delta.closed.
   rewrite* sch_subst_fresh.
   apply* typing_cst.
-  rewrite* <- (sch_subst_fresh _ H2).
-  destruct (Delta.type c) as [T Ks]; simpl in *.
+  rewrite* <- (sch_subst_fresh TS H2).
   apply* proper_instance_well_subst.
   (* GC *)
   apply* (@typing_gc gc (List.map (kind_subst S) Ks)
@@ -605,24 +637,21 @@ Proof.
   simpl. destruct a. simpl. rewrite H. rewrite* IHE.
 Qed.
 
-Lemma map_sch_subst_extend : forall S S0 E,
+Lemma map_sch_subst_extend : forall S HS S0 HS0 E,
   extends S S0 ->
-  map (sch_subst S) (map (sch_subst S0) E) = map (sch_subst S) E.
+  map (@sch_subst S HS) (map (@sch_subst S0 HS0) E) = map (sch_subst HS) E.
 Proof.
   intros.
   apply map_compose.
   intros.
-  destruct a as [T Ks]; unfold sch_subst; simpl.
-  rewrite* (H T).
-  apply (f_equal (Sch (typ_subst S T))).
-  induction Ks; simpl*.
+  destruct a as [T Ks HM]; apply sch_eq; simpl*.
+  clear HM; induction Ks; simpl*.
   rewrite IHKs.
   rewrite* (@kind_subst_combine S).
 Qed.
 
 Lemma kenv_ok_sch_kinds : forall K M Xs,
   kenv_ok K ->
-  scheme M ->
   fresh (dom K) (sch_arity M) Xs ->
   kenv_ok (K & kinds_open_vars (sch_kinds M) Xs).
 Proof.
@@ -634,10 +663,10 @@ Proof.
   apply env_prop_concat. apply (proj2 H).
   unfold kinds_open_vars, kinds_open.
   apply list_forall_env_prop.
-  destruct* (H0 Xs).
-  clear -H3; induction H3. simpl*.
+  destruct* (sch_ok M Xs).
+  clear -H2; induction H2. simpl*.
   simpl; constructor; auto.
-  unfold kind_open. unfold typ_open_vars in H3.
+  unfold kind_open. unfold typ_open_vars in H2.
   apply* All_kind_types_map.
 Qed.
 
@@ -702,29 +731,27 @@ Hint Resolve well_subst_extends.
 
 Definition Gc := (false, GcLet).
 
-Definition soundness_spec h t K0 E T Ts S0 K S :=
-  typinf K0 E t T Ts S0 h = Some (K, S) ->
-  is_subst S0 -> env_prop type S0 ->
-  kenv_ok K0 -> disjoint (dom S0) (dom K0) ->
-  env_ok E -> type T ->
-  extends S S0 /\ env_prop type S /\ is_subst S /\
-  kenv_ok K /\ disjoint (dom S) (dom K) /\
-  well_subst K0 (map (kind_subst S) K) S /\
-  map (kind_subst S) K; map (sch_subst S) E |Gc|= t ~: typ_subst S T.
+Definition soundness_spec h t K0 E T Ts S0 (TS0:env_prop type S0) K S :=
+  typinf K0 (strip_env E) t T Ts S0 h = Some (K, S) ->
+  is_subst S0 -> kenv_ok K0 -> disjoint (dom S0) (dom K0) ->
+  ok E -> type T ->
+  exists TS,
+    extends S S0 /\ is_subst S /\ kenv_ok K /\ disjoint (dom S) (dom K) /\
+    well_subst K0 (map (kind_subst S) K) S /\
+    map (kind_subst S) K; map (@sch_subst S TS) E |Gc|= t ~: typ_subst S T.
 
-Lemma soundness_ind : forall h t K0 E T Ts S0 K S s x,
-  scheme s ->
-  fresh (fvs S0 K0 E T Ts) (sch_arity s) x ->
+Lemma soundness_ind : forall h t K0 E T Ts S0 TS0 K S s x,
+  fresh (fvs S0 K0 (strip_env E) T Ts) (sch_arity s) x ->
   unify (K0 & kinds_open_vars (sch_kinds s) x) (sch_open_vars s x) T S0 =
     Some (K, S) ->
   (kenv_ok (K0 & kinds_open_vars (sch_kinds s) x) ->
    extends S S0 -> kenv_ok K ->
    unifies S ((sch_open_vars s x, T) :: nil) ->
    map (kind_subst S0) (K0 & kinds_open_vars (sch_kinds s) x);
-   map (sch_subst S0) E |Gc|= t ~: sch_subst S0 s ^^ typ_fvars x) ->
-  soundness_spec h t K0 E T Ts S0 K S.
+   map (@sch_subst S0 TS0) E |Gc|= t ~: sch_subst TS0 s ^^ typ_fvars x) ->
+  soundness_spec h t K0 E T Ts TS0 K S.
 Proof.
-  intros until x; intros Hs f HI Typ _ HS0 HTS0 HK0 Dis HE HT.
+  intros until x. intros f HI Typ _ HS0 HK0 Dis HE HT.
   unfold unify in HI.
   assert (kenv_ok (K0 & kinds_open_vars (sch_kinds s) x)).
     apply* kenv_ok_sch_kinds.
@@ -739,18 +766,19 @@ Proof.
     inversions H2; clear H2.
     split*.
     unfold sch_open_vars.
-    destruct* (Hs x).
+    destruct* (sch_ok s x).
+  exists (proj1 H3).
   intuition.
       destruct* (unify_keep _ _ _ HI).
     intro; intros.
     apply H5.
     apply* binds_concat_ok.
-  rewrite <- (map_sch_subst_extend E Hext).
+  rewrite <- (map_sch_subst_extend (proj1 H3) TS0 E Hext).
   use (unify_types _ _ _ HI HS0).
-  rewrite* <- (H7 (sch_open_vars s x) T).
+  rewrite* <- (H6 (sch_open_vars s x) T).
   rewrite* <- Hext.
   unfold fvs in f.
-  rewrite* sch_subst_open_vars.
+  rewrite* (sch_subst_open_vars TS0).
   poses Hkext (fun k => sym_eq (kind_subst_combine _ _ _ k Hext)).
   rewrite (map_map_env _ _ _ K Hkext).
   apply* typing_typ_well_subst.
@@ -778,24 +806,37 @@ Proof.
   intros. rewrite* kind_subst_open_vars.
 Qed.
 
-Lemma soundness_var : forall h Ts v K0 E T S0 K S,
-  soundness_spec (Datatypes.S h) (trm_fvar v) K0 E T Ts S0 K S.
+Lemma binds_strip : forall x p E,
+  binds x p (strip_env E) ->
+  exists M, binds x M E /\ fst p = sch_type M /\ snd p = sch_kinds M.
 Proof.
-  intros; intros HI HS0 HTS0 HK0 Dis HE HT.
+  unfold binds; induction E; simpl; intros. discriminate.
+  destruct a; simpl in *.
+  destruct* (x == v).
+  inversions H.
+  esplit; split*.
+Qed.
+
+Lemma soundness_var : forall h Ts v K0 E T S0 TS0 K S,
+  @soundness_spec (Datatypes.S h) (trm_fvar v) K0 E T Ts S0 TS0 K S.
+Proof.
+  intros; intros HI HS0 HK0 Dis HE HT.
   poses HI' HI; simpl in HI.
-  case_rewrite (get v E) R1.
-  destruct (var_freshes (fvs S0 K0 E T Ts) (sch_arity s));
+  set (E0 := strip_env E) in *.
+  case_rewrite (get v E0) R1.
+  destruct (var_freshes (fvs S0 K0 E0 T Ts) (length (snd p)));
     simpl proj1_sig in HI.
   unfold fvs in f.
-  refine (soundness_ind _ _ _ _ _ HI _ HI' _ _ _ _ _ _); auto.
-    apply (proj2 HE _ _ (binds_in R1)).
+  destruct (binds_strip E R1) as [[T1 Ks HM] [BM [HMT HMKs]]].
+  rewrite HMT in *; rewrite HMKs in *.
+  refine (soundness_ind _ _ TS0 _ _ _ HI _ HI' _ _ _ _ _); auto.
   intros.
   apply* typing_var.
     apply* kenv_ok_map.
   split.
-    simpl; rewrite map_length.
-    rewrite (fresh_length _ _ _ f). apply types_typ_fvars.
-  destruct s as [Us Ks]; simpl.
+    unfold sch_arity. simpl. rewrite map_length.
+    simpl in f. rewrite (fresh_length _ _ _ f). apply types_typ_fvars.
+  simpl.
   apply* well_kinded_open_vars.
 Qed.
 
@@ -818,15 +859,15 @@ Proof.
   intro; use (H x).
 Qed.
 
-Lemma soundness_cst : forall h Ts c K0 E T S0 K S,
-  soundness_spec (Datatypes.S h) (trm_cst c) K0 E T Ts S0 K S.
+Lemma soundness_cst : forall h Ts c K0 E T S0 TS0 K S,
+  @soundness_spec (Datatypes.S h) (trm_cst c) K0 E T Ts S0 TS0 K S.
 Proof.
-  intros; intros HI HS0 HTS0 HK0 Dis HE HT.
+  intros; intros HI HS0 HK0 Dis HE HT.
   poses HI' HI; simpl in HI.
-  destruct (var_freshes (fvs S0 K0 E T Ts) (sch_arity (Delta.type c)));
+  set (E0 := strip_env E) in *.
+  destruct (var_freshes (fvs S0 K0 E0 T Ts) (sch_arity (Delta.type c)));
     simpl in HI.
-  refine (soundness_ind _ _ _ _ _ HI _ HI' _ _ _ _ _ _); auto.
-    apply Delta.scheme.
+  refine (soundness_ind _ _ TS0 _ _ _ HI _ HI' _ _ _ _ _); auto.
   intros.
   rewrite sch_subst_fresh; try (rewrite Delta.closed; intro; auto).
   apply* typing_cst.
@@ -835,7 +876,7 @@ Proof.
     rewrite (fresh_length _ _ _ f). apply types_typ_fvars.
   pattern (sch_kinds (Delta.type c)) at 2.
   rewrite <- (kinds_subst_cst S0 c).
-  unfold fvs in f.
+  unfold fvs, sch_arity in f.
   apply* well_kinded_open_vars.
 Qed.
 
@@ -857,14 +898,15 @@ Proof.
   simpl. destruct* (x1 == x1).
 Qed.
 
-Lemma soundness_abs : forall h Ts t K0 E T S0 S K,
-  (forall t K0 E T Ts S0 K S, soundness_spec h t K0 E T Ts S0 K S) ->
-  soundness_spec (Datatypes.S h) (trm_abs t) K0 E T Ts S0 K S.
+Lemma soundness_abs : forall h Ts t K0 E T S0 TS0 S K,
+  (forall t K0 E T Ts S0 TS0 K S, @soundness_spec h t K0 E T Ts S0 TS0 K S) ->
+  @soundness_spec (Datatypes.S h) (trm_abs t) K0 E T Ts S0 TS0 K S.
 Proof.
-  intros until K; intros IHh  HI HS0 HTS0 HK0 Dis HE HT; simpl in HI.
-  destruct (var_fresh (fvs S0 K0 E T Ts)); simpl in HI.
-  destruct (var_fresh (fvs S0 K0 E T Ts \u {{x}})); simpl in HI.
-  destruct (var_fresh (dom E \u trm_fv t)); simpl in HI.
+  intros until K; intros IHh  HI HS0 HK0 Dis HE HT; simpl in HI.
+  set (E0 := strip_env E) in *.
+  destruct (var_fresh (fvs S0 K0 E0 T Ts)); simpl in HI.
+  destruct (var_fresh (fvs S0 K0 E0 T Ts \u {{x}})); simpl in HI.
+  destruct (var_fresh (dom E0 \u trm_fv t)); simpl in HI.
   case_rewrite (unify K0 (typ_arrow (typ_fvar x) (typ_fvar x0)) T S0) R1.
   destruct p as [K' S'].
   unfold unify in R1.
@@ -873,28 +915,39 @@ Proof.
     simpl; intros. destruct* H.
     inversions* H.
   destruct* (unify_kinds_ok _ _ R1). clear H1; destruct H2.
-  destruct* (IHh _ _ _ _ _ _ _ _ HI); clear IHh HI.
-    env_fix. split; auto.
-    apply* env_prop_concat.
-    apply env_prop_single.
-    intro; intros. unfold typ_open_vars. simpl*.
+  assert ((x1, (typ_fvar x, nil)) :: E0 =
+          strip_env ((x1, Sch_nil (type_fvar x))::E)) by reflexivity.
+  unfold presch in HI; rewrite H3 in HI; clear H3.
+  destruct* (IHh _ _ _ _ _ _ (proj1 H0) _ _ HI); clear IHh HI.
+Lemma dom_strip_env : forall E, dom (strip_env E) = dom E.
+Proof.
+  induction E; simpl*.
+  destruct a; simpl. rewrite* IHE.
+Qed.
+    unfold E0 in n1; rewrite dom_strip_env in n1.
+    apply* ok_cons.
+  exists x2.
   intuition.
       apply* extends_trans.
       apply* typ_subst_extend.
     apply* well_subst_compose.
   use (unify_types _ _ _ R1 HS0).
-  rewrite <- (H3 T).
-  rewrite* <- (H10 (typ_arrow (typ_fvar x) (typ_fvar x0)) T).
-  rewrite H3.
+  rewrite <- (H0 T).
+  rewrite* <- (H9 (typ_arrow (typ_fvar x) (typ_fvar x0)) T).
+  rewrite H0.
   simpl.
-  simpl map in H11.
   fold (typ_subst S (typ_fvar x0)).
   fold (typ_subst S (typ_fvar x)).
-  set (E' := map (sch_subst S) E) in *.
+  env_fix. rewrite map_concat in H10.
+  set (E' := map (sch_subst x2) E) in *.
   apply* (@typing_abs Gc (dom E' \u {{x1}} \u trm_fv t)).
+  instantiate (1:=typ_subst_type x2 (type_fvar x)).
   intros.
   apply typing_gc_raise.
   apply* (@typing_abs_rename x1).
+  replace (Sch_nil (typ_subst_type x2 (type_fvar x)))
+    with (sch_subst x2 (Sch_nil (type_fvar x))) by apply* sch_eq.
+  auto.
 Qed.
 
 Lemma incl_subset_dom : forall (A:Set) (E1 E2:env A),
@@ -956,8 +1009,9 @@ Qed.
 Lemma scheme_generalize : forall Bs Ks T,
   length Bs = length Ks ->
   type T -> list_forall (All_kind_types type) Ks ->
-  scheme (sch_generalize Bs T Ks).
+  let (T', Ks') := sch_generalize Bs T Ks in typ_body T' Ks'.
 Proof.
+  unfold sch_generalize.
   intros.
   intro; simpl; intros.
   rewrite map_length in H2.
@@ -1071,13 +1125,6 @@ Proof.
   use (IHInA _ Hx). auto with sets.
 Qed.
 
-Lemma sch_arity_subst : forall M S,
-  sch_arity (sch_subst S M) = sch_arity M.
-Proof.
-  destruct M as [T Ks]; simpl.
-  intro; rewrite* map_length.
-Qed.
-
 Hint Resolve kind_subst_idem.
 
 Lemma disjoint_subset : forall L1 L2 L3,
@@ -1121,10 +1168,10 @@ Proof.
 Qed.
 
 Lemma sch_generalize_disjoint : forall Bs T Ks,
-  disjoint (sch_fv (sch_generalize Bs T Ks)) (mkset Bs).
+  disjoint (pre_fv (sch_generalize Bs T Ks)) (mkset Bs).
 Proof.
   intros.
-  unfold sch_generalize, sch_fv; simpl.
+  unfold sch_generalize, pre_fv; simpl.
   apply disjoint_union. apply typ_generalize_disjoint.
   apply kinds_generalize_disjoint.
 Qed.
@@ -1205,20 +1252,38 @@ Definition ok_concat_inv1 A (E1 E2:env A) H := proj1 (ok_concat_inv E1 E2 H).
 Definition ok_concat_inv2 A (E1 E2:env A) H := proj2 (ok_concat_inv E1 E2 H).
 Hint Immediate ok_concat_inv1 ok_concat_inv2.
 
-Lemma typing_let_fresh : forall T1 l l0 K' e e0 e1 e2 fvT1 fvE,
+Lemma sch_fv_pre_fv : forall T Ks HM,
+  sch_fv (@Sch T Ks HM) = pre_fv (T, Ks).
+Proof.
+  intros; reflexivity.
+Qed.
+
+Lemma fv_in_strip_env : forall E,
+  fv_in pre_fv (strip_env E) = env_fv E.
+Proof.
+  unfold env_fv; induction E; simpl*.
+  destruct a. rewrite IHE. reflexivity.
+Qed.
+
+Lemma typing_let_fresh : forall T1 l l0 K' e e0 e1 e2 fvT1 fvE M,
   let ftve := close_fvk K' fvE in
   let Bs := S.elements (S.diff fvT1 (ftve \u dom e2)) in
   let l0' := List.map (fun _:var => @None ckind) Bs in
-  let M := sch_generalize (@app var l Bs) T1 (@app kind l0 l0') in
+  strip_pre M = sch_generalize (@app var l Bs) T1 (@app kind l0 l0') ->
   split e2 = (l, l0) ->
   ok (e0 & e) -> ok (e2 & e1) ->
   ok K' -> incl (e0 & e) K' -> incl (e2 & e1) e ->
   disjoint ftve (dom e) ->
   dom e0 << ftve ->
-  fresh (fvE \u sch_fv M \u dom e0 \u fv_in kind_fv e0) (sch_arity M) (l++Bs).
+  fresh (fvE \u sch_fv M \u dom e0 \u fv_in kind_fv e0)
+    (sch_arity M) (l++Bs).
 Proof.
-  intros until M. intros R4 Ok Ok' HK' Inc2 Inc4 Dise Se0.
-  simpl length. rewrite map_length. rewrite app_length.
+  intros until l0'. intros RM R4 Ok Ok' HK' Inc2 Inc4 Dise Se0.
+  destruct M as [T Ks HM]. inversion RM; clear RM.
+  rewrite sch_fv_pre_fv.
+  unfold sch_arity; simpl.
+  pattern Ks at 2; rewrite H1.
+  rewrite map_length. rewrite app_length.
   rewrite <- (split_length _ R4).
   use (split_combine e2). rewrite R4 in H.
   apply fresh_app.
@@ -1227,17 +1292,17 @@ Proof.
   rewrite* <- (dom_combine l l0).
   rewrite H.
   use (incl_subset_dom Inc4).
-  rewrite dom_concat in H0.
+  rewrite dom_concat in H2.
   assert (dom e2 << dom e).
-    intros v Hv. apply* (H0 v).
-  use (disjoint_subset H1
+    intros v Hv. apply* (H2 v).
+  use (disjoint_subset H3
           (typing_let_disjoint _ _ _ Ok HK' Inc2 Dise Se0)).
-  assert (disjoint (sch_fv M) (dom e2)).
-    unfold M.
+  assert (disjoint (pre_fv (T,Ks)) (dom e2)).
+    subst T Ks.
     rewrite <- H.
     rewrite* dom_combine.
     use(sch_generalize_disjoint (l++Bs) T1 (l0 ++ l0')).
-    rewrite mkset_app in H3.
+    rewrite mkset_app in H0. unfold sch_generalize in H0.
     disjoint_solve.
   disjoint_solve.
   unfold l0'.
@@ -1249,12 +1314,13 @@ Proof.
   puts (diff_disjoint fvT1 (ftve \u mkset l)).
   set (l' := S.diff fvT1 (ftve \u mkset l)) in *.
   assert (disjoint ftve l') by disjoint_solve.
-  puts (typing_let_disjoint _ _ _ Ok HK' Inc2 H1 Se0).
-  clear H1.
-  assert (disjoint (sch_fv M) l').
-    unfold M.
+  puts (typing_let_disjoint _ _ _ Ok HK' Inc2 H3 Se0).
+  clear H3.
+  assert (disjoint (pre_fv (T, Ks)) l').
+    subst T Ks.
     use(sch_generalize_disjoint (l++Bs) T1 (l0 ++ l0')).
-    rewrite mkset_app in H1.
+    unfold sch_generalize in H0.
+    rewrite mkset_app in H0.
     rewrite <- (mkset_elements l').
     unfold l'.
     rewrite <- (dom_combine l l0).
@@ -1274,7 +1340,6 @@ Qed.
 
 Lemma typing_let_fresh_2 : forall l1 l2 K' T fvE e e0 e1 e2,
   let Ks := List.map (kind_map (typ_generalize l1)) l2 in
-  let M' := Sch T Ks in
   kenv_ok K' ->  ok (e0 & e) -> ok (e2 & e1) ->
   incl (e0 & e) K' -> incl (e2 & e1) e ->
   split e1 = (l1, l2) ->
@@ -1282,13 +1347,13 @@ Lemma typing_let_fresh_2 : forall l1 l2 K' T fvE e e0 e1 e2,
   dom e0 << close_fvk K' fvE ->
   disjoint (close_fvk K' (typ_fv T)) (dom e1) ->
   dom e2 << close_fvk K' (typ_fv T) ->
-  fresh (fvE \u sch_fv M' \u dom (e0 & e2) \u fv_in kind_fv (e0 & e2))
-    (sch_arity M') l1.
+  fresh (fvE \u pre_fv (T,Ks) \u dom (e0 & e2) \u fv_in kind_fv (e0 & e2))
+    (length Ks) l1.
 Proof.
-  intros until M'.
+  intros until Ks.
   intros HK' Ok Ok' Inc2 Inc4 R5 Dise Se0 Dise1 Se2.
   rewrite dom_concat; rewrite fv_in_concat.
-  simpl length.
+  unfold sch_arity; simpl length.
   unfold Ks; rewrite map_length.
   rewrite <- (split_length _ R5).
   poses He1 (split_combine e1). rewrite R5 in He1.
@@ -1304,8 +1369,8 @@ Proof.
          (typing_let_disjoint _ _ _ Ok (proj1 HK') Inc2 Dise Se0)).
   apply disjoint_comm.
   repeat apply disjoint_union; try solve [disjoint_solve].
-  (* sch_fv M' *)
-  unfold sch_fv; simpl.
+  (* pre_fv *)
+  unfold pre_fv; simpl.
   apply disjoint_union.
     apply* disjoint_subset. apply close_fvk_subset.
   unfold Ks.
@@ -1321,15 +1386,15 @@ Proof.
     apply* in_dom.
   apply* in_ok_binds.
   apply Inc2.
-  apply in_or_concat; left.
+  apply in_or_concat; right.
   apply* Inc4.
 Qed.
 
-Lemma sch_open_extra : forall Ks Xs T,
-  type T -> sch_open_vars (Sch T Ks) Xs = T.
+Lemma sch_open_extra : forall T Ks HM Xs,
+  type T -> sch_open_vars (@Sch T Ks HM) Xs = T.
 Proof.
   unfold sch_open_vars, typ_open_vars; simpl; intros.
-  rewrite* <- typ_open_type.
+  apply* typ_open_type.
 Qed.
 
 Lemma typing_let_incl : forall K' e e0 e1 e2 : kenv,
@@ -1378,7 +1443,7 @@ Proof.
       apply list_forall_env_prop.
       unfold l0'; clear; induction Bs; simpl*.
     rewrite He2. intro; intros. apply (proj2 HK' x).
-    apply Inc2. apply in_or_concat; left. apply* Inc4.
+    apply Inc2. apply in_or_concat; right. apply* Inc4.
   rewrite dom_concat. rewrite He2.
   apply disjoint_comm; apply disjoint_union.
     rewrite dom_combine.
@@ -1393,17 +1458,18 @@ Proof.
   intro; intros. apply* Inc4.
 Qed.
 
-Lemma soundness_generalize : forall L K' E' t T1 KA M,
+Lemma soundness_generalize : forall L K' E' t T1 KA T Ks,
   K'; E' |Gc|= t ~: T1 ->
-  typinf_generalize K' E' L T1 = (KA, M) ->
-  kenv_ok KA /\ incl KA K' /\ S.inter (dom K') L << dom KA /\ scheme M /\
-  exists L1, forall Xs,
-    fresh L1 (sch_arity M) Xs ->
-    KA & kinds_open_vars (sch_kinds M) Xs; E' |(true,GcLet)|= t ~: M ^ Xs.
+  typinf_generalize K' (strip_env E') L T1 = (KA, (T, Ks)) ->
+  kenv_ok KA /\ incl KA K' /\ S.inter (dom K') L << dom KA /\
+  exists HM, exists L1, forall Xs,
+    fresh L1 (sch_arity (@Sch T Ks HM)) Xs ->
+    KA & kinds_open_vars (sch_kinds (Sch HM)) Xs; E'
+      |(true,GcLet)|= t ~: Sch HM ^ Xs.
 Proof.
   unfold typinf_generalize.
   introv Typ HI.
-  set (ftve := close_fvk K' (env_fv E')) in *.
+  set (ftve := close_fvk K' (fv_in pre_fv (strip_env E'))) in *.
   case_rewrite (split_env ftve K') R2.
   case_rewrite (split_env (close_fvk K' (typ_fv T1)) e) R3.
   case_rewrite (split e2) R4.
@@ -1424,8 +1490,8 @@ Proof.
         apply Inc2. apply* in_or_concat.
       rewrite* He2.
     unfold l0'. clear; induction Bs; simpl*.
-  assert (HM: scheme M).
-    subst M; unfold l0'.
+  assert (HM: typ_body T Ks).
+    subst T Ks; unfold l0'.
     apply* scheme_generalize.
     do 2 rewrite app_length. rewrite map_length. rewrite* (split_length _ R4).
   assert (IncKA: incl (e0 & e4) K').
@@ -1452,25 +1518,27 @@ Proof.
     rewrite dom_concat in H.
     sets_solve.
     destruct* (Dise3 a).
-  split. rewrite* H1.
-  intros.
-  assert (AryM: sch_arity M = length (l ++ Bs)).
-    rewrite <- H1.
-    simpl. unfold l0'.
+  rewrite H1. rewrite H2.
+  exists HM.
+  assert (AryM: sch_arity (Sch HM) = length (l ++ Bs)).
+    unfold sch_arity; simpl. rewrite <- H2; unfold l0'.
     autorewrite with list.
     rewrite* (split_length _ R4).
   esplit; intros.
   apply typing_weaken_kinds.
   eapply typing_rename_typ.
       instantiate (1 := l ++ Bs).
-      unfold l0', Bs, ftve; apply* typing_let_fresh.
+      rewrite <- fv_in_strip_env.
+      unfold l0', Bs, ftve.
+      apply* typing_let_fresh.
+      instantiate (1:=T1). unfold strip_pre. simpl. subst T Ks. reflexivity.
     instantiate (1 := dom (e0 & e4) \u mkset (l++Bs)) in H.
     rewrite dom_concat in H.
-    rewrite <- AryM; rewrite* <- H1.
+    rewrite* <- AryM.
   unfold sch_open_vars, typ_open_vars. simpl sch_type.
-  rewrite* typ_generalize_reopen.
+  subst T. rewrite* typ_generalize_reopen.
   unfold sch_generalize. simpl sch_kinds.
-  rewrite* kinds_generalize_reopen.
+  subst Ks. rewrite* kinds_generalize_reopen.
   rewrite* combine_app.
   fold (@combine var kind Bs l0' & combine l l0).
   rewrite <- concat_assoc.
@@ -1482,25 +1550,35 @@ Proof.
   apply* (@typing_gc (true,GcLet) Ks). simpl*.
   poses Typ' (typing_gc_raise Typ). clear Typ. simpl in Typ'.
   intros.
-  pose (M' := Sch T1 Ks).
-  rewrite* <- (@sch_open_extra Ks Xs0). fold M'.
+  assert (Hl2: list_forall (All_kind_types type) l2).
+    apply* env_prop_list_forall.
+      rewrite He1. intro; intros. apply* (proj2 HK' x).
+      apply Inc2. apply* in_or_concat.
+    rewrite* He1.
+  assert (HM': typ_body T1 Ks).
+    assert (HT1: type T1) by auto.
+    split. unfold typ_open_vars.
+      clear -HT1; induction HT1; simpl*.
+    puts (scheme_generalize l1 (split_length _ R6) HT1 Hl2).
+    unfold sch_generalize in H2.
+    destruct (H2 Xs1 H1).
+    apply H4.
+  pose (M' := Sch HM').
+  rewrite* <- (sch_open_extra HM' Xs0). fold M'.
   replace Ks with (sch_kinds M') by simpl*.
   eapply typing_rename_typ.
       instantiate (1 := l1).
       unfold M', Ks.
       unfold ftve in *.
-      apply* (@typing_let_fresh_2 l1 l2 K').
+      rewrite sch_fv_pre_fv.
+      apply* (@typing_let_fresh_2 l1 l2 K'). rewrite* <- fv_in_strip_env.
+      rewrite* <- fv_in_strip_env.
     unfold Ks in H0. rewrite map_length in H0.
     rewrite* (split_length _ R6).
-  assert (list_forall (All_kind_types type) l2).
-    apply* env_prop_list_forall.
-      rewrite He1. intro; intros. apply* (proj2 HK' x).
-      apply Inc2. apply* in_or_concat.
-    rewrite* He1.
   simpl sch_kinds.
-  unfold Ks; rewrite* kinds_generalize_reopen. rewrite He1; clear H2.
+  unfold Ks; rewrite* kinds_generalize_reopen. rewrite He1.
   unfold sch_open_vars, typ_open_vars.
-  simpl sch_type. rewrite* <- typ_open_type.
+  simpl sch_type. rewrite* typ_open_type.
   destruct* (typing_let_incl _ _ _ Ok Ok' Inc1 Inc2 Inc3 Inc4).
   apply* typing_kenv_incl.
   split.
@@ -1510,7 +1588,7 @@ Proof.
     eapply disjoint_subset. apply (incl_subset_dom Inc4).
     apply disjoint_comm. apply* ok_disjoint.
   intro; intros. apply* (proj2 (proj1 (typing_regular Typ')) x).
-  apply* kenv_ok_sch_kinds. rewrite* H1.
+  apply* kenv_ok_sch_kinds.
 Qed.
 
 Lemma well_subst_let_inf: forall K0 s k e S K,
@@ -1542,78 +1620,102 @@ Proof.
   puts (S.singleton_2 (refl_equal x)). auto with sets.
 Qed.
 
-Lemma soundness_let : forall h Ts t1 t2 K0 E T S0 S K,
-  (forall t K0 E T Ts S0 K S, soundness_spec h t K0 E T Ts S0 K S) ->
-  soundness_spec (Datatypes.S h) (trm_let t1 t2) K0 E T Ts S0 K S.
+Lemma soundness_let : forall h Ts t1 t2 K0 E T S0 TS0 S K,
+  (forall t K0 E T Ts S0 TS0 K S, @soundness_spec h t K0 E T Ts S0 TS0 K S) ->
+  @soundness_spec (Datatypes.S h) (trm_let t1 t2) K0 E T Ts S0 TS0 K S.
 Proof.
-  intros until K; intros IHh  HI HS0 HTS0 HK0 Dis HE HT; simpl in HI.
-  destruct (var_fresh (fvs S0 K0 E T Ts)); simpl in HI.
-  case_rewrite (typinf K0 E t1 (typ_fvar x) (T::Ts) S0 h) R1. destruct p.
+  intros until K; intros IHh HI HS0 HK0 Dis HE HT; simpl in HI.
+  set (E0 := strip_env E) in *.
+  destruct (var_fresh (fvs S0 K0 E0 T Ts)); simpl in HI.
+  case_rewrite (typinf K0 E0 t1 (typ_fvar x) (T::Ts) S0 h) R1. destruct p.
   fold (typ_subst s (typ_fvar x)) in HI.
   set (K' := map (kind_subst s) k) in *.
-  set (E' := map (sch_subst s) E) in *.
+  destruct* (IHh _ _ _ _ _ _ TS0 _ _ R1)
+    as [HTs [Hext [Hs [Hk [Disk [WS' Typ']]]]]]; clear R1.
+  pose (E' := map (sch_subst HTs) E).
+  set (E0' := map (pre_subst s) E0) in *.
+Lemma strip_sch_subst : forall S TS M,
+  strip_pre (@sch_subst S TS M) = pre_subst S (strip_pre M).
+Proof.
+  intros. destruct M; reflexivity.
+Qed.
+Lemma strip_env_subst : forall S TS E,
+  strip_env (map (@sch_subst S TS) E) = map (pre_subst S) (strip_env E).
+Proof.
+  induction E; simpl*.
+  destruct a. simpl. rewrite IHE. rewrite* strip_sch_subst.
+Qed.
   set (T1 := typ_subst s (typ_fvar x)) in *.
-  destruct (var_fresh (dom E \u trm_fv t1 \u trm_fv t2)); simpl proj1_sig in HI.
-  case_rewrite (typinf_generalize K' E' (vars_subst s (dom K0)) T1) R2.
-  destruct* (IHh _ _ _ _ _ _ _ _ R1); clear R1.
-  destruct H0 as [HTs [Hs [Hk [Disk [WS' Typ']]]]].
+  destruct (var_fresh (dom E0 \u trm_fv t1 \u trm_fv t2));
+    simpl proj1_sig in HI.
+  case_rewrite (typinf_generalize K' E0' (vars_subst s (dom K0)) T1) R2.
+  unfold E0',E0,K' in R2. rewrite <- (strip_env_subst HTs) in R2.
+  destruct p as [T0 Ks].
   destruct (soundness_generalize _ Typ' R2)
     as [HKA [Inc2 [Inc1 [HM [L Typ2]]]]].
-  destruct* (IHh _ _ _ _ _ _ _ _ HI); clear IHh HI.
-      use (incl_subset_dom Inc2).
-      rewrite dom_map in H0.
-      intro v; destruct* (Disk v).
-    env_fix. split; auto.
+  unfold presch in HI.
+  replace ((x0,(T0,Ks))::E0) with (strip_env ((x0,Sch HM)::E))
+    in HI by reflexivity.
+  destruct* (IHh _ _ _ _ _ _ HTs _ _ HI); clear IHh HI.
+        use (incl_subset_dom Inc2).
+        rewrite dom_map in H.
+        intro v; destruct* (Disk v).
+      unfold E0 in n0; rewrite dom_strip_env in n0.
+      apply* ok_cons.
+  exists x1.
   intuition.
       apply* extends_trans.
     apply* well_subst_let_inf.
-  apply* (@typing_let Gc (sch_subst S s0) (dom S \u dom K \u L)).
+  apply* (@typing_let Gc (sch_subst x1 (Sch HM)) (dom S \u dom K \u L)).
     intros.
-    simpl.
+    simpl sch_kinds.
     rewrite* <- kinds_subst_open_vars.
     rewrite* <- sch_subst_open_vars.
-    rewrite sch_arity_subst in H6.
-    rewrite <- (map_sch_subst_extend E H0).
+    rewrite sch_subst_arity in H4.
+    rewrite <- (map_sch_subst_extend x1 HTs E H0).
     apply* typing_typ_well_subst.
-      apply (well_subst_extend (sch_kinds s0) Xs H2 H5).
-      rewrite* dom_map.
+      apply (well_subst_extend (sch_kinds (Sch HM)) Xs x1 H3).
+      unfold sch_arity in H4; rewrite* dom_map.
     rewrite <- map_concat.
     apply* kenv_ok_map.
+    replace Ks with (sch_kinds (Sch HM)) by reflexivity.
     apply* kenv_ok_sch_kinds.
   intros.
-  instantiate (1 := dom E \u trm_fv t2 \u {{x0}}) in H6.
+  instantiate (1 := dom E \u trm_fv t2 \u {{x0}}) in H4.
   apply typing_gc_raise.
   apply* (@typing_abs_rename x0).
   rewrite* dom_map.
 Qed.
 
-Lemma soundness_app : forall h Ts t1 t2 K0 E T S0 S K,
-  (forall t K0 E T Ts S0 K S, soundness_spec h t K0 E T Ts S0 K S) ->
-  soundness_spec (Datatypes.S h) (trm_app t1 t2) K0 E T Ts S0 K S.
+Lemma soundness_app : forall h Ts t1 t2 K0 E T S0 TS0 S K,
+  (forall t K0 E T Ts S0 TS0 K S, @soundness_spec h t K0 E T Ts S0 TS0 K S) ->
+  @soundness_spec (Datatypes.S h) (trm_app t1 t2) K0 E T Ts S0 TS0 K S.
 Proof.
-  intros until K; intros IHh HI HS0 HTS0 HK0 Dis HE HT; simpl in HI.
-  destruct (var_fresh (fvs S0 K0 E T Ts)); simpl in HI.
-  case_rewrite (typinf K0 E t1 (typ_arrow (typ_fvar x) T) Ts S0 h) R1.
+  intros until K; intros IHh HI HS0 HK0 Dis HE HT; simpl in HI.
+  set (E0 := strip_env E) in *.
+  destruct (var_fresh (fvs S0 K0 E0 T Ts)); simpl in HI.
+  case_rewrite (typinf K0 E0 t1 (typ_arrow (typ_fvar x) T) Ts S0 h) R1.
   destruct p as [K' S'].
-  destruct* (IHh _ _ _ _ _ _ _ _ R1); clear R1.
-  destruct* (IHh _ _ _ _ _ _ _ _ HI); clear IHh HI.
+  destruct* (IHh _ _ _ _ _ _ TS0 _ _ R1); clear R1.
+  destruct* (IHh _ _ _ _ _ _ x0 _ _ HI); clear IHh HI.
+  exists x1.
   intuition.
       apply* extends_trans.
     apply* well_subst_compose.
   remember (typ_fvar x) as T1.
   apply* typing_app.
-  use (well_subst_extends H1 H10).
-  use (typing_typ_well_subst H0 H11 (kenv_ok_map H6 H0) H12).
-  rewrite (map_sch_subst_extend E H1) in H14.
-  rewrite H1 in H14.
-  apply H14.
+  use (well_subst_extends H H8).
+  use (typing_typ_well_subst x1 H9 (kenv_ok_map H4 x1) H10).
+  rewrite (map_sch_subst_extend x1 x0 E H) in H12.
+  rewrite H in H12.
+  apply H12.
 Qed.
 
-Theorem typinf_sound : forall h t K0 E T Ts S0 K S,
-  soundness_spec h t K0 E T Ts S0 K S.
+Theorem typinf_sound : forall h t K0 E T Ts S0 TS0 K S,
+  @soundness_spec h t K0 E T Ts S0 TS0 K S.
 Proof.
   induction h; destruct t; intros;
-    intros HI HS0 HTS0 HK0 Dis HE HT; try discriminate.
+    intros HI HS0 HK0 Dis HE HT; try discriminate.
   apply* (soundness_var h Ts).
   apply* (@soundness_abs h Ts).
   apply* (@soundness_let h Ts).
@@ -1720,6 +1822,7 @@ Proof.
   simpl. congruence.
 Qed.
 
+(*
 Lemma unifies_open : forall S n Us L Xs M0 T,
   env_prop type S ->
   types n Us ->
@@ -1745,6 +1848,7 @@ Proof.
     auto.
   intros y Hy; auto with sets.
 Qed.
+*)
 
 Lemma kind_subst_intro0 : forall S Xs Us k, 
   fresh (kind_fv k) (length Xs) Xs -> 
@@ -1766,7 +1870,8 @@ Lemma fv_in_sch : forall Xs M,
   fv_in kind_fv (combine Xs (sch_kinds M)) << sch_fv M.
 Proof.
   intros.
-  destruct M as [T Ks]. unfold sch_fv; simpl.
+  destruct M as [T Ks HM]. unfold sch_fv; simpl.
+  clear HM.
   gen Ks; induction Xs; simpl; intros. auto.
   destruct Ks; simpl in *; auto.
   use (IHXs Ks).
@@ -1793,20 +1898,20 @@ Proof.
   unfold fvs; use (binds_dom H).
 Qed.
 
-Lemma well_subst_concat_abs : forall K M0 Us S S0 K0 E T Ts Xs x,
-  env_prop type S ->
-  dom S << fvs S0 K0 E T Ts ->
-  proper_instance K (sch_kinds (sch_subst S M0)) Us ->
+Lemma well_subst_concat_abs : forall K M0 Us S TS S0 K0 E T Ts Xs x,
+  let E0 := strip_env E in
+  dom S << fvs S0 K0 E0 T Ts ->
+  proper_instance K (@sch_subst S TS M0) Us ->
   well_subst (map (kind_subst S0) K0) K S ->
   binds x M0 E ->
-  fresh (fvs S0 K0 E T Ts) (sch_arity M0) Xs ->
+  fresh (fvs S0 K0 E0 T Ts) (sch_arity M0) Xs ->
   sch_arity M0 = length Us ->
-  (forall t, typ_fv t << fvs S0 K0 E T Ts ->
+  (forall t, typ_fv t << fvs S0 K0 E0 T Ts ->
     typ_subst (S & combine Xs Us) t = typ_subst S t) ->
   extends (S & combine Xs Us) S0 ->
   well_subst (K0 & kinds_open_vars (sch_kinds M0) Xs) K (S & combine Xs Us).
 Proof.
-  intros until x; intros HTS HS [HUs HWk] WS B Fr AryM Hsub Hext'.
+  intros until E0; intros HS [HUs HWk] WS B Fr AryM Hsub Hext'.
   intro; intros.
   binds_cases H.
     apply* (well_subst_concat _ _ WS Hsub Hext').
@@ -1828,14 +1933,15 @@ Proof.
       use (fv_in_sch Xs M0).
       rewrite <- (fresh_length _ _ _ Fr).
       apply* fresh_sub.
-      unfold fvs, env_fv; intros y Hy; simpl in *; sets_solve.
-    rewrite sch_arity_subst in HUs.
+      unfold fvs; intros y Hy; simpl in *; sets_solve.
+      unfold E0; rewrite fv_in_strip_env. unfold env_fv; auto.
+    rewrite sch_subst_arity in HUs.
     rewrite* <- (fresh_length _ _ _ Fr).
   unfold kinds_open_vars, kinds_open in B1.
   elim (get_none_notin _ H).
   use (binds_dom B1).
   rewrite dom_combine. rewrite dom_combine in H0. auto.
-  rewrite map_length. rewrite* (fresh_length _ _ _ Fr).
+  rewrite map_length. unfold sch_arity in Fr; rewrite* (fresh_length _ _ _ Fr).
   rewrite <- AryM. rewrite* (fresh_length _ _ _ Fr).
 Qed.
 
@@ -2003,7 +2109,7 @@ Qed.
 Definition moregen_scheme K M0 M :=
   forall Ys, fresh (dom K) (sch_arity M) Ys ->
     exists Ts,
-      proper_instance (K & kinds_open_vars (sch_kinds M) Ys) (sch_kinds M0) Ts
+      proper_instance (K & kinds_open_vars (sch_kinds M) Ys) M0 Ts
       /\ sch_open M0 Ts = sch_open M (typ_fvars Ys).
 
 Definition moregen_env K E0 E :=
@@ -2255,11 +2361,12 @@ Proof.
 Qed.
 *)
 
-Lemma sch_fv_subst : forall S M,
-  sch_fv (sch_subst S M) << sch_fv M \u fv_in typ_fv S.
+Lemma sch_fv_subst : forall S TS M,
+  sch_fv (@sch_subst S TS M) << sch_fv M \u fv_in typ_fv S.
 Proof.
-  destruct M as [T Ks].
+  destruct M as [T Ks HM].
   unfold sch_fv, sch_subst; simpl.
+  clear HM.
   sets_solve.
     use (typ_fv_subst S _ H).
   induction Ks; simpl in *. auto.
@@ -2276,15 +2383,15 @@ Proof.
   use (IHKs H _ Hy).
 Qed.
 
-Lemma proper_instance_inf : forall K M Us Ys M' Vs M0 S,
-  proper_instance K (sch_kinds M) Us ->
-  proper_instance (K & kinds_open_vars (sch_kinds M) Ys) (sch_kinds M') Vs ->
+Lemma proper_instance_inf : forall K M Us Ys M' Vs M0 S TS,
+  proper_instance K M Us ->
+  proper_instance (K & kinds_open_vars (sch_kinds M) Ys) M' Vs ->
   fresh (dom K \u fv_in kind_fv K \u sch_fv M \u sch_fv M0 \u fv_in typ_fv S)
     (sch_arity M) Ys ->
-  sch_subst S M0 = M' ->
-  proper_instance K (sch_kinds M') (List.map (typ_subst (combine Ys Us)) Vs).
+  @sch_subst S TS M0 = M' ->
+  proper_instance K M' (List.map (typ_subst (combine Ys Us)) Vs).
 Proof.
-  intros until S; intros [HUs WUs] [HVs WVs] FrYs HM0.
+  intros until TS; intros [HUs WUs] [HVs WVs] FrYs HM0.
   split.
     apply* typ_subst_type_list.
     apply list_forall_env_prop.
@@ -2317,7 +2424,7 @@ Proof.
       apply* fresh_sub.
     apply* well_kinded_subst.
     apply well_subst_open_vars.
-          auto.
+          unfold sch_arity in FrYs. auto.
         unfold sch_fv in FrYs.
         apply* (fresh_resize (sch_arity M)).
       rewrite* <- (fresh_length _ _ _ FrYs).
@@ -2331,6 +2438,7 @@ Proof.
   apply disjoint_comm.
   apply (fresh_disjoint (sch_arity M)).
   rewrite <- HM0 in H.
+  destruct M0 as [T0 K0 M0].
   unfold sch_subst in H; simpl in H.
   destruct (proj1 (in_map_iff (kind_subst S) _ _) H) as [k1 [Hk1 Bk1]].
   subst x.
@@ -2340,23 +2448,24 @@ Proof.
   apply* fresh_sub.
 Qed.
 
-Lemma sch_open_inf : forall M Us S M0 Vs Ys,
+Lemma sch_open_inf : forall M Us S TS M0 Vs Ys,
   types (sch_arity M) Us ->
-  sch_open (sch_subst S M0) Vs = sch_open M (typ_fvars Ys) ->
+  sch_open (sch_subst TS M0) Vs = sch_open M (typ_fvars Ys) ->
   fresh (sch_fv M \u sch_fv M0 \u fv_in typ_fv S) (sch_arity M) Ys ->
-  sch_open (sch_subst S M0) (List.map (typ_subst (combine Ys Us)) Vs) =
+  sch_open (@sch_subst S TS M0) (List.map (typ_subst (combine Ys Us)) Vs) =
   sch_open M Us.
 Proof.
   introv HUs EVs FrYs.
   assert (HTUs: env_prop type (combine Ys Us)).
     apply list_forall_env_prop.
     apply (proj2 HUs).
-  replace (sch_subst S M0) with (sch_subst (combine Ys Us) (sch_subst S M0)).
+  replace (sch_subst TS M0) with (sch_subst HTUs (sch_subst TS M0)).
     rewrite* <- sch_subst_open.
     rewrite EVs.
     rewrite (proj1 HUs) in FrYs.
-    rewrite* sch_subst_open.
+    rewrite* (sch_subst_open HTUs).
     rewrite* (fresh_subst _ _ Us FrYs).
+    destruct M as [T Ks M].
     unfold sch_open, sch_subst; simpl.
     rewrite* typ_subst_fresh.
     rewrite dom_combine.
@@ -2367,92 +2476,115 @@ Proof.
   rewrite* sch_subst_fresh.
   rewrite dom_combine.
     apply disjoint_comm.
-    apply (disjoint_subset (@sch_fv_subst S M0) (L3:=mkset Ys)).
+    apply (disjoint_subset (sch_fv_subst TS M0) (L3:=mkset Ys)).
     apply* (fresh_disjoint (sch_arity M)).
   rewrite <- (fresh_length _ _ _ FrYs).
   apply (proj1 HUs).
 Qed.
 
-Definition principality S0 K0 E0 S K E t T Ts h :=
+Definition principality S0 K0 E0 S TS K E t T Ts h :=
+  let E0' := strip_env E0 in
   is_subst S0 -> env_prop type S0 ->
   kenv_ok K0 -> disjoint (dom S0) (dom K0) ->
-  env_ok E0 -> moregen_env K (map (sch_subst S) E0) E ->
-  env_prop type S -> dom S << fvs S0 K0 E0 T Ts ->
+  ok E0 -> moregen_env K (map (@sch_subst S TS) E0) E ->
+  dom S << fvs S0 K0 E0' T Ts ->
   extends S S0 -> well_subst K0 K S ->
   K; E |(false,GcAny)|= t ~: typ_subst S T ->
   trm_depth t < h ->
   exists K', exists S',
-    typinf K0 E0 t T Ts S0 h = Some (K', S') /\
-    extends S' S0 /\ fvs S0 K0 E0 T Ts << fvs S' K' E0 T Ts /\
+    typinf K0 E0' t T Ts S0 h = Some (K', S') /\
+    extends S' S0 /\ fvs S0 K0 E0' T Ts << fvs S' K' E0' T Ts /\
     exists S'',
-      dom S'' << S.diff (fvs S' K' E0 T Ts) (fvs S0 K0 E0 T Ts) /\
+      dom S'' << S.diff (fvs S' K' E0' T Ts) (fvs S0 K0 E0' T Ts) /\
       extends (S & S'') S' /\
       well_subst K' K (S & S'').
 
-Lemma principal_var : forall h Ts S0 K0 E0 S K E x T,
-  principality S0 K0 E0 S K E (trm_fvar x) T Ts (Datatypes.S h).
+Check list_ind.
+
+Lemma env_ind : forall (A:Set) (P:env A -> Prop),
+  P empty -> (forall x a E, P E -> P (E & x ~ a)) ->
+  forall E, P E.
 Proof.
-  intros; intros HS0 HTS0 HK0 Dis HE0 MGE HTS HS Hext WS Typ Hh.
+  induction E. apply H.
+  destruct a.
+  apply (H0 v a _ IHE).
+Qed.
+
+Lemma strip_binds : forall x M E,
+  binds x M E -> binds x (strip_pre M) (strip_env E).
+Proof.
+  induction E using env_ind; intros. elim (binds_empty H).
+  simpl. env_fix.
+  binds_cases H; auto*. subst*.
+Qed.
+
+Lemma principal_var : forall h Ts S0 K0 E0 S TS K E x T,
+  @principality S0 K0 E0 S TS K E (trm_fvar x) T Ts (Datatypes.S h).
+Proof.
+  intros; intros HS0 HTS0 HK0 Dis OkE0 MGE HS Hext WS Typ Hh.
   inversions Typ; clear Typ; try discriminate.
   simpl.
   destruct (proj2 MGE _ _ H5) as [M' [B' MGM]].
   destruct (binds_map_inv _ _ B') as [M0 [HM0 B]].
-  rewrite B.
-  destruct (var_freshes (fvs S0 K0 E0 T Ts) (sch_arity M0)) as [Xs Fr]; simpl.
+  rewrite (strip_binds B).
+  set (E0' := strip_env E0) in *.
+  destruct (var_freshes (fvs S0 K0 E0' T Ts) (sch_arity M0)) as [Xs Fr]; simpl.
   destruct (var_freshes (dom K \u fv_in kind_fv K \u sch_fv M \u sch_fv M0
               \u fv_in typ_fv S) (sch_arity M)) as [Ys FrYs].
-  destruct* (MGM Ys) as [Vs [HVs EVs]]. destruct* H6.
+  destruct* (MGM Ys) as [Vs [HVs EVs]].
   pose (Vs' := List.map (typ_subst (combine Ys Us)) Vs).
   assert (AryM0: sch_arity M0 = length Vs').
-    destruct HVs. subst. rewrite sch_arity_subst in H4.
-    unfold Vs'; rewrite map_length. apply (proj1 H4).
-  assert (Hsub: forall t, typ_fv t << fvs S0 K0 E0 T Ts ->
+    destruct HVs. subst. rewrite sch_subst_arity in H.
+    unfold Vs'; rewrite map_length. apply (proj1 H).
+  assert (Hsub: forall t, typ_fv t << fvs S0 K0 E0' T Ts ->
                   typ_subst (S & combine Xs Vs') t = typ_subst S t).
     rewrite AryM0 in Fr.
     intros.
     apply* typ_subst_combine_fresh.
     apply* fresh_sub.
   assert (Ok: ok (K0 & kinds_open_vars (sch_kinds M0) Xs)).
-    unfold fvs in Fr. 
-    apply* ok_kinds_open_vars.
+    apply* disjoint_ok. unfold kinds_open_vars. apply* ok_combine_fresh.
+    rewrite* dom_kinds_open_vars.
+     unfold fvs in Fr.
+    apply* (fresh_disjoint (sch_arity M0)).
   assert (Hext': extends (S & combine Xs Vs') S0).
     clear -Fr Hext Hsub.
     apply* extends_concat. unfold fvs; intros x Hx; auto with sets.
-  assert (PI: proper_instance K (sch_kinds M') Vs').
-    unfold Vs' in *. apply* proper_instance_inf. split*.
+  assert (PI: proper_instance K M' Vs')
+    by (unfold Vs' in *; apply* proper_instance_inf).
   assert (HU: unifies (S & combine Xs Vs') ((sch_open_vars M0 Xs, T) :: nil)).
     subst.
     unfold unifies; simpl; intros.
-    destruct* H4. inversions H4; clear H4.
-    destruct HVs. rewrite sch_arity_subst in H4.
+    destruct* H. inversions H; clear H.
+    destruct HVs. rewrite sch_subst_arity in H.
     apply* unifies_open.
         unfold Vs'.
         apply* typ_subst_type_list.
         apply* list_forall_env_prop.
-        apply (proj2 H).
+        apply (proj2 (proj1 H6)).
       intros y Hy.
       use (fv_in_spec sch_fv _ _ _ (binds_in B)).
       unfold fvs, env_fv; simpl*.
     rewrite <- H0.
-    unfold Vs'. apply* (sch_open_inf _ _ _ _ _ H EVs).
+    unfold Vs'. apply* (sch_open_inf _ _ _ _ _ (proj1 H6) EVs).
   case_eq
     (unify (K0 & kinds_open_vars (sch_kinds M0) Xs) (sch_open_vars M0 Xs) T S0);
     unfold unify; intros.
     destruct p as [K' S']. esplit; esplit. split*.
     unfold fvs in Fr.
-    destruct* (unify_mgu0 (K':=K) (S':=S & combine Xs Vs') _ H4).
+    destruct* (unify_mgu0 (K':=K) (S':=S & combine Xs Vs') _ H).
       intro; intros.
       subst M'.
       apply* (well_subst_concat_abs Xs HTS HS PI (x:=x)).
-    destruct* (unify_kinds_ok _ _ H4).
+    destruct* (unify_kinds_ok _ _ H).
       rewrite dom_concat.
       rewrite* dom_kinds_open_vars.
       disjoint_solve.
     split.
-      apply (typ_subst_extend _ _ _ HS0 H4).
-    puts (unify_keep_fv _ _ H4 HS0 Ok (E:=E0) (T:=T) (Ts:=Ts)).
+      apply (typ_subst_extend _ _ _ HS0 H).
+    puts (unify_keep_fv _ _ H HS0 Ok (E:=E0) (T:=T) (Ts:=Ts)).
     split.
-      intros y Hy; apply H10; clear -Hy.
+      intros y Hy; apply H9; clear -Hy.
       unfold fvs in *.
       rewrite dom_concat; rewrite* fv_in_concat.
     exists (combine Xs Vs').
@@ -2460,14 +2592,14 @@ Proof.
     intros y Hy.
     rewrite dom_combine in Hy.
       apply S.diff_3.
-        apply H10.
+        apply H9.
         unfold fvs.
         rewrite dom_concat.
         rewrite* dom_kinds_open_vars.
       destruct* (fresh_disjoint _ _ _ Fr y).
     rewrite* <- (fresh_length _ _ _ Fr).
   elimtype False.
-  refine (unify_complete0 (K:=K) HS0 Ok Hext' HU _ _ H4).
+  refine (unify_complete0 (K:=K) HS0 Ok Hext' HU _ _ H).
     subst; apply* well_subst_concat_abs.
   omega.
 Qed.
@@ -2562,7 +2694,7 @@ Lemma principal_abs : forall h Ts S0 K0 E0 S K E t1 T,
   principality S0 K0 E0 S K E (trm_abs t1) T Ts (Datatypes.S h).
 Proof.
   intros until T.
-  intros IHh HS0 HTS0 HK0 Dis HE0 MGE HTS HS Hext WS Typ Hh.
+  intros IHh HS0 HTS0 HK0 Dis HE0 OkE0 MGE HTS HS Hext WS Typ Hh.
   simpl.
   destruct (var_fresh (fvs S0 K0 E0 T Ts)) as [x1 Fr1]; simpl.
   destruct (var_fresh (fvs S0 K0 E0 T Ts \u {{x1}})) as [x2 Fr2]; simpl.
@@ -2609,7 +2741,6 @@ Proof.
     destruct* (IHh (T::Ts) S' K' (E0 & x ~ Sch (typ_fvar x1) nil)
                    (S & combine Xs Us) K (E & x ~ Sch U nil)
                    (t1 ^ x) (typ_fvar x2)).
-          split; auto.
           apply* env_prop_concat. intro; intros.
           destruct H9; inversions H9.
           apply* type_scheme.
@@ -2973,7 +3104,7 @@ Proof.
 Qed.
 
 Lemma moregen_scheme_fv : forall K M0 M,
-  moregen_scheme K M0 M ->
+  moregen_scheme K M0 M -> scheme M ->
   sch_fv M0 << sch_fv M \u fv_in kind_fv K.
 Proof.
   unfold moregen_scheme.
@@ -2985,27 +3116,27 @@ Proof.
   unfold sch_fv in Hy; simpl in Hy; sets_solve.
     unfold sch_open in SO; simpl in SO.
     puts (typ_fv_open (typ_fvars Ys) T2).
-    rewrite <- SO in H1.
+    rewrite <- SO in H2.
     puts (typ_fv_open_min Ts T1).
     unfold sch_fv; simpl.
     sets_solve.
     unfold sch_fv in Fr; simpl in Fr.
-    destruct (fresh_disjoint _ _ _ Fr y). elim H2; auto.
-    rewrite typ_fv_typ_fvars in H1. elim (H2 H1).
-  unfold proper_instance in PI. intuition.
+    destruct (fresh_disjoint _ _ _ Fr y). elim H3; auto.
+    rewrite typ_fv_typ_fvars in H2. elim (H3 H2).
+  unfold proper_instance in PI. intuition. simpl in H5.
   unfold sch_fv; simpl.
   unfold sch_fv in Fr; simpl in Fr.
-  clear -Fr H0 H2.
+  clear -Fr H1 H5.
   remember Ts as Us.
-  pattern Us at 2 in H2. rewrite HeqUs in H2.
-  clear HeqUs; gen Ts; induction K1; intros. elim (in_empty H0).
+  pattern Us at 2 in H5. rewrite HeqUs in H5.
+  clear HeqUs; gen Ts; induction K1; intros. elim (in_empty H1).
   simpl in *. destruct* Ts.
-  destruct H2.
+  destruct H5.
   sets_solve.
     inversions H. destruct a; try discriminate. elim (in_empty H2).
     puts (kind_fv_open_min Us a).
     puts (kind_entails_fv (Some k') (Some k)).
-    simpl in H6; rewrite H0 in H6.
+    simpl in H6; rewrite H1 in H6.
     puts (H6 H5); sets_solve.
     puts (fv_in_spec kind_fv _ _ _ (binds_in H3) Hin0).
     rewrite fv_in_concat in H4.
@@ -3013,7 +3144,7 @@ Proof.
     unfold kinds_open_vars in H7.
     rewrite fv_in_kind_fv_list in H7.
       clear -Fr H2 H7.
-      set (n := length K2) in Fr.
+      set (n := sch_arity (Sch T2 K2)) in Fr.
       clearbody n; gen n; induction K2; intros. elim (in_empty H7).
       simpl in *.
       sets_solve.
@@ -3030,10 +3161,10 @@ Proof.
 Qed.
 
 Lemma moregen_env_fv : forall K E E0,
-  moregen_env K E0 E -> ok E0 ->
+  moregen_env K E0 E -> ok E0 -> env_prop scheme E ->
   env_fv E0 << env_fv E \u fv_in kind_fv K.
 Proof.
-  introv HME Ok.
+  introv HME Ok HSE.
   destruct HME.
   intros y Hy.
   destruct (fv_in_binds sch_fv E0 Hy) as [x [a [Hx B]]].
@@ -3042,7 +3173,7 @@ Proof.
   destruct (dom_binds _ H1) as [z Hz].
   destruct (H0 _ _ Hz) as [b [Hb HM]].
   puts (binds_func Hb (in_ok_binds _ _ B Ok)). subst b.
-  use (moregen_scheme_fv HM).
+  use (moregen_scheme_fv HM (HSE _ _ (binds_in Hz))).
   sets_solve.
   unfold env_fv.
   use (fv_in_spec sch_fv _ _ _ (binds_in Hz)).
@@ -3085,7 +3216,7 @@ Theorem typinf_principal : forall h Ts S0 K0 E0 S K E t T,
   principality S0 K0 E0 S K E t T Ts h.
 Proof.
   induction h; intros until T;
-    intros HS0 HTS0 HK0 Dis HE0 MGE HTS HS Hext WS Typ Hh;
+    intros HS0 HTS0 HK0 Dis HE0 OkE0 MGE HTS HS Hext WS Typ Hh;
     try (elimtype False; omega).
   inversions Typ.
   apply* (@principal_var h Ts S0 K0 E0 S K E).
@@ -3096,7 +3227,7 @@ Lemma principal_let : forall h Ts S0 K0 E0 S K E t1 t2 T,
   principality S0 K0 E0 S K E (trm_let t1 t2) T Ts (Datatypes.S h).
 Proof.
   intros until T.
-  intros IHh HS0 HTS0 HK0 Dis HE0 MGE HTS HS Hext WS Typ Hh.
+  intros IHh HS0 HTS0 HK0 Dis HE0 OkE0 MGE HTS HS Hext WS Typ Hh.
   simpl.
   destruct (var_fresh (fvs S0 K0 E0 T Ts)) as [x1 Fr1]; simpl.
   destruct (var_fresh (dom E0 \u trm_fv t1 \u trm_fv t2)) as [x Frx]; simpl.
@@ -3133,12 +3264,15 @@ Proof.
         destruct* (MGM1 Ys).
         exists x2.
         split*.
-        destruct H1. destruct H1.
-        split*.
+        destruct H2. destruct H2.
+        split*. split*.
+        destruct H4.
         apply* For_all2_imp.
         intros. apply* well_kinded_weaken.
         rewrite <- dom_concat in H0.
-        apply* ok_kinds_open_vars.
+        apply* disjoint_ok.
+          unfold kinds_open_vars. apply* ok_combine_fresh.
+        rewrite* dom_kinds_open_vars. apply* fresh_disjoint.
       intros. apply Hsub. unfold fvs; auto.
      rewrite Hcb.
      apply* well_subst_concat.
@@ -3190,13 +3324,12 @@ Proof.
     unfold l0'; clear. induction Bs; simpl*.
   destruct* (IHh Ts S' e0 (E0 & x ~ M0) (S & x1 ~ MXs) K (E & x~M) (t2 ^ x) T)
     as [K'' [S1' [HI' [Hext'' [Hfvs'' [S1'' H1'']]]]]].
-           destruct* (kenv_ok_concat_inv _ _ Oke).
-          intuition.
-          intro y; destruct (H14 y). auto.
-          poses Hs (incl_subset_dom H16).
-          unfold K1 in Hs; rewrite dom_map in Hs.
-          use (notin_subset Hs H17).
-         split*.
+          destruct* (kenv_ok_concat_inv _ _ Oke).
+         intuition.
+         intro y; destruct (H14 y). auto.
+         poses Hs (incl_subset_dom H16).
+         unfold K1 in Hs; rewrite dom_map in Hs.
+         use (notin_subset Hs H17).
         split.
           repeat rewrite dom_concat.
           rewrite <- (proj1 MGE). repeat rewrite dom_map.
@@ -3227,7 +3360,7 @@ Lemma moregen_let :
   let l0' := List.map (fun _ : var => None) Bs in
   let M0 := sch_generalize (l++Bs) T1 (l0++l0') in
   moregen_env K (map (sch_subst S) E0) E ->
-  env_ok E0 ->
+  env_prop scheme E -> ok E0 ->
   split_env ftve K1 = (e, e0) ->
   split_env (close_fvk K1 (typ_fv T1)) e = (e1, e2) ->
   split e2 = (l, l0) ->
@@ -3244,7 +3377,7 @@ Lemma moregen_let :
   moregen_scheme K (sch_subst (S & x1 ~ MXs) M0) M.
 Proof.
   intros until M0.
-  intros MGE OkE0 R1 R2 R3 HS'' Hext Fr Fr1 HS' HTS' HTS HTS''
+  intros MGE HSE OkE0 R1 R2 R3 HS'' Hext Fr Fr1 HS' HTS' HTS HTS''
     Oke0 Oke2 Ok' WS Typ.
   intro; intros.
   assert (type T1) by (unfold T1; auto).
@@ -3253,21 +3386,21 @@ Proof.
   assert (env_prop type (S & x1 ~ MXs & S'')) by apply* env_prop_concat.
   cut (x1 \in sch_fv M0 -> M0 = Sch (typ_fvar x1) nil /\ x1 \in ftve);
     intros.
-  (*  unfold M0 in H3; simpl in H3.
+  (*  unfold M0 in H4; simpl in H4.
     case_eq (get x1 S'); introv R4.
       assert (x1 \notin close_fvk K1 (typ_fv T1)).
         puts (binds_dom R4).
         unfold T1; simpl; rewrite R4; simpl; intro.
-        destruct (S.union_1 (close_fvk_inv _ _ H5)).
-          unfold K1 in H6.
-          destruct (S.union_1 (fv_in_kind_subst _ _ H6)).
-            elim (S.diff_2 H7 H4).
-          clear -H4 HS' H7.
+        destruct (S.union_1 (close_fvk_inv _ _ H6)).
+          unfold K1 in H7.
+          destruct (S.union_1 (fv_in_kind_subst _ _ H7)).
+            elim (S.diff_2 H8 H5).
+          clear -H5 HS' H8.
           unfold is_subst in HS'.
           assert (env_prop (fun T => x1 \notin typ_fv T) S').
             intro; intros. intro.
             destruct* (HS' _ _ H x1).
-          clear -H7 H; induction S'. elim (in_empty H7).
+          clear -H8 H; induction S'. elim (in_empty H8).
           simpl in *. destruct a.
           assert (x1 \notin typ_fv t) by apply* (H v t).
           elim IHS'. sets_solve. elim (H0 H1).
@@ -3275,46 +3408,46 @@ Proof.
         destruct* (HS' _ _ (binds_in R4) x1).
       destruct (split_env_ok _ R2).
         destruct* (ok_concat_inv _ _ (proj1 Oke0)).
-      use (sch_fv_generalize H3).
-      unfold sch_fv in H7; simpl in H7.
-      destruct (S.union_1 H7); clear H7.
-        elim (H4 (close_fvk_subset _ H8)).
-      rewrite kind_fv_list_app in H8.
+      use (sch_fv_generalize H4).
+      unfold sch_fv in H8; simpl in H8.
       destruct (S.union_1 H8); clear H8.
-        rewrite <- (fv_in_kind_fv_list _ _ (split_length _ R3)) in H7.
-        use (split_combine e2). rewrite R3 in H8. rewrite H8 in H7.
-        destruct (fv_in_binds _ _ H7) as [y [b [Hx Hy]]].
+        elim (H5 (close_fvk_subset _ H9)).
+      rewrite kind_fv_list_app in H9.
+      destruct (S.union_1 H9); clear H9.
+        rewrite <- (fv_in_kind_fv_list _ _ (split_length _ R3)) in H8.
+        use (split_combine e2). rewrite R3 in H9. rewrite H9 in H8.
+        destruct (fv_in_binds _ _ H8) as [y [b [Hx Hy]]].
         assert (HK1: ok K1) by (unfold K1; auto).
         destruct* (split_env_ok _ R1). 
-        elim H4; clear H4.
+        elim H5; clear H5.
         assert (In (y,b) K1).
-          apply (proj44 H10).
-          apply in_or_concat; left*.
+          apply (proj44 H11).
+          apply in_or_concat; right*.
         refine (close_fvk_ok _ _ _ _ Hx); trivial.
-          apply (proj42 H6). apply (in_dom _ _ _ Hy).
+          apply (proj42 H7). apply (in_dom _ _ _ Hy).
         auto.
-      unfold l0' in H7.
-      elimtype False; clear -H7; induction Bs. elim (in_empty H7).
+      unfold l0' in H8.
+      elimtype False; clear -H8; induction Bs. elim (in_empty H8).
       simpl in *. elim IHBs. sets_solve. elim (in_empty H).
     unfold T1 in *.
     unfold M0. simpl. rewrite R4.
     simpl in R2; rewrite R4 in R2; simpl in R2.
     destruct (split_env_ok _ R2).
       destruct* (ok_concat_inv _ _ (proj1 Oke0)).
-    use (split_combine e2). rewrite R3 in H6.
+    use (split_combine e2). rewrite R3 in H7.
     assert (x1 \in ftve).
       case_eq (S.mem x1 ftve); intros; auto with sets.
-      puts (mem_3 H7); clear H7.
-      simpl in H3; rewrite R4 in H3.
+      puts (mem_3 H8); clear H8.
+      simpl in H4; rewrite R4 in H4.
       destruct* (sch_generalize_disjoint (l++Bs) (typ_fvar x1) (l0 ++ l0') x1).
-      elim H7; clear H7.
+      elim H8; clear H8.
       rewrite mkset_app.
       unfold Bs; rewrite mkset_elements.
       simpl; rewrite R4; simpl.
-      rewrite <- H6. rewrite dom_combine.
+      rewrite <- H7. rewrite dom_combine.
         case_eq (S.mem x1 (mkset l)); intros; auto with sets.
         assert (x1 \in close_fvk K1 {{x1}}) by apply* close_fvk_subset.
-        use (mem_3 H7).
+        use (mem_3 H8).
       apply* split_length.
     split*.
     destruct (split_env_ok _ R1).
@@ -3322,42 +3455,42 @@ Proof.
     assert (close_fvk K1 {{x1}} << ftve).
       unfold ftve.
       apply close_fvk_ok2. unfold K1; auto.
-      intro; intros. rewrite <- (S.singleton_1 H10).
-      apply H7.
+      intro; intros. rewrite <- (S.singleton_1 H11).
+      apply H8.
     assert (l = nil).
       destruct* l.
       destruct e2. discriminate.
       destruct p.
-      simpl in H5.
+      simpl in H6.
       assert (v \in ftve).
-        apply* H10.
-      use (incl_subset_dom (proj44 H5)).
-      rewrite dom_concat in H12.
-      simpl in H12.
+        apply* H11.
+      use (incl_subset_dom (proj44 H6)).
+      rewrite dom_concat in H13.
+      simpl in H13.
       assert (v \in dom e) by auto.
-      destruct* ((proj41 H9) v).
-    rewrite H11.
+      destruct* ((proj41 H10) v).
+    rewrite H12.
     case_eq Bs; intros.
-      destruct l0. unfold l0'. rewrite H12.
+      destruct l0. unfold l0'. rewrite H13.
         unfold sch_generalize; simpl*.
-      puts (split_length _ R3). rewrite H11 in H13; discriminate.
-    assert (SetoidList.InA S.E.eq e3 Bs) by rewrite* H12.
-    puts (S.elements_2 H13).
-    elim (S.diff_2 H14).
-    simpl in H14; rewrite R4 in H14. simpl in H14. auto. *)
+      puts (split_length _ R3). rewrite H12 in H14; discriminate.
+    assert (SetoidList.InA S.E.eq e3 Bs) by rewrite* H13.
+    puts (S.elements_2 H14).
+    elim (S.diff_2 H15).
+    simpl in H15; rewrite R4 in H15. simpl in H15. auto. *)
   case_eq (S.mem x1 (sch_fv M0)); introv R4.
-    destruct (H3 (S.mem_2 R4)).
+    destruct (H4 (S.mem_2 R4)).
     assert (typ_fv MXs << close_fvk K (env_fv E \u fv_in kind_fv K)).
       poses WS1 (well_subst_extends Hext WS). fold K1 in WS1.
       assert (ok (K & kinds_open_vars (sch_kinds M) Xs)) by auto.
-      puts (@close_fvk_subst _ _ _ x1 E1 WS1 H6 H5).
-      unfold typ_subst in H7.
-      rewrite (binds_concat_fresh (x:=x1) (a:=MXs)) in H7.
-        unfold E1 in H7. rewrite map_sch_subst_extend in H7; auto.
-        rewrite <- (env_subst_ext_fv S) in H7.
+      puts (@close_fvk_subst _ _ _ x1 E1 WS1 H7 H6).
+      unfold typ_subst in H8.
+      rewrite (binds_concat_fresh (x:=x1) (a:=MXs)) in H8.
+        unfold E1 in H8. rewrite map_sch_subst_extend in H8; auto.
+        rewrite <- (env_subst_ext_fv S) in H8.
           sets_solve.
           assert (ok (map (sch_subst S) E0)) by auto.
-          puts (moregen_env_fv MGE H7).
+          puts (moregen_env_fv MGE H8 HSE).
           unfold MXs in Hy. unfold sch_open_vars, typ_open_vars in Hy.
           refine (close_fvk_disjoint _ (kinds_open_vars (sch_kinds M) Xs)
                     _ _ _).
@@ -3386,14 +3519,17 @@ Proof.
          use (mem_3 R1).
         auto.
        intro.
-       elim (S.diff_2 (HS'' _ H8)).
+       elim (S.diff_2 (HS'' _ H9)).
        unfold fvs; simpl*.
-    rewrite H4.
+    rewrite H5.
     unfold sch_subst; simpl. destruct* (x1 == x1). clear e3.
     exists (@nil typ).
     split.
       unfold MXs.
       split. split*.
+      split. intro; intros. destruct Xs0; try discriminate.
+        simpl. split*. unfold typ_open_vars.
+        rewrite <- typ_open_type; apply* sch_open_vars_type.
       unfold kinds_open; simpl*.
     unfold sch_open; simpl.
     rewrite <- typ_open_type; try apply* sch_open_vars_type.
@@ -3401,7 +3537,7 @@ Proof.
       apply* fresh_sub.
       sets_solve.
       use (close_fvk_inv _ _ Hin).
-    clear -H7 H.
+    clear -H8 H.
     unfold MXs in *.
     unfold sch_open_vars, typ_open_vars in *.
     clear MXs; induction (sch_type M); simpl*.
@@ -3409,17 +3545,17 @@ Proof.
         destruct* n.
         destruct* Ys. elim H.
       destruct* n.
-      destruct H7.
+      destruct H8.
       destruct Ys. elim H.
       destruct n0. elim H0. simpl*.
       simpl. apply (IHXs n Ys). simpl in H. destruct* H.
       simpl*.
-    simpl in H7.
+    simpl in H8.
     rewrite* IHt1.
     rewrite* IHt2.
-   auto.
-  clear H3.
-  unfold M0, T1.
+   unfold MXs.
+   destruct* (H0 Xs).
+
 Qed.
 
 End Mk2.
